investigations/bedrock2/Constants.v
@@ -1,0 +1,23 @@
+Require Import Coq.Strings.String.
+Require Import Coq.ZArith.ZArith.
+Require Import bedrock2.Syntax.
+Require Import coqutil.Word.Interface.
+
+Module constant.
+  (* Typeclass for constant values *)
+  Definition constant (name : string) : Type := Z.
+  Existing Class constant.
+
+  (* Typeclass for functions that convert a constant to a bedrock2 expression *)
+  Definition interp : Type := forall name, constant name -> expr.expr.
+  Existing Class interp.
+
+  (* Use `Existing Instance constants.var_interp` to interpret constants as
+     named variables -- useful for printing C that will use those constants *)
+  Definition var_interp : interp := fun name _ => expr.var name.
+
+  (* Use `Existing Instance constants.literal_interp` to interpret constants as
+     literals -- useful for proofs *)
+  Definition literal_interp : interp := fun _ => expr.literal.
+End constant.
+Notation constant := constant.constant.
