investigations/bedrock2/IncrementWait/IncrementWaitToC.v
@@ -2,20 +2,28 @@ Require Import Coq.Lists.List.
 Require Import Coq.ZArith.ZArith.
 Require Import bedrock2.ToCString.
 Require Import coqutil.Z.HexNotation.
+Require Import Bedrock2Experiments.Constants.
 Require Import Bedrock2Experiments.IncrementWait.IncrementWaitSemantics.
 Require Import Bedrock2Experiments.IncrementWait.IncrementWait.
 Import ListNotations.
+Local Open Scope Z_scope.
 
 Definition BASE_ADDR : Z := Ox"1000".
 
-Instance consts : constants :=
-  {| constants.STATUS_IDLE := 0;
-     constants.STATUS_BUSY := 1;
-     constants.STATUS_DONE := 2;
-     constants.STATUS_ADDR := BASE_ADDR + Ox"0";
-     constants.VALUE_ADDR := BASE_ADDR + Ox"4";
+Instance env : global_env :=
+  {| global_env.STATUS_IDLE := 0;
+     global_env.STATUS_BUSY := 1;
+     global_env.STATUS_DONE := 2;
+     global_env.STATUS_ADDR := BASE_ADDR + Ox"0";
+     global_env.VALUE_ADDR := BASE_ADDR + Ox"4";
   |}.
 
-Definition funcs := [put_wait_get].
+Definition funcs {interp : constant.interp} := [put_wait_get].
+
+(* Print with constants as variables *)
+Existing Instance constant.var_interp.
+
+(* Uncomment to print with constants as literals *)
+(* Existing Instance constant.literal_interp. *)
 
 Redirect "incrementwait.c" Compute c_module funcs.
